theories/tests/swap.v
@@ -1,0 +1,28 @@
+From iris_c.clang Require Import logic notations tactics.
+
+Section example.
+  Context `{clangG Σ}.
+
+  Definition x: ident := 1.
+
+  Definition Edecl (t: type) (x: ident) e : expr :=
+    Elet_typed t x (Ealloc t (Evalue (default_val t))) e.
+    
+  Definition swap (t: type) (l1 l2: addr) :=
+    Edecl t x
+    (x <- ! l1 @ t ;; l1 <- !l2 @ t ;; l2 <- x).
+
+  Lemma swap_spec t l1 l2 v1 v2 Φ :
+    l1 ↦ v1 @ t ∗ l2 ↦ v2 @ t ∗
+    (l1 ↦ v2 @ t -∗ l2 ↦ v1 @ t -∗ Φ void)
+    ⊢ WP swap t l1 l2 {{ Φ }}.
+  Proof.
+    iIntros "(Hl1 & Hl2 & HΦ)".
+    rewrite /swap /Edecl.
+    iDestruct (mapsto_typeof with "Hl1") as "%".
+    iDestruct (mapsto_typeof with "Hl2") as "%".
+    wp_alloc lx as "Hlx". wp_let.
+    wp_run. iApply ("HΦ" with "Hl1 Hl2").
+  Qed.
+  
+End example.
